@prefix bibo: <http://purl.org/ontology/bibo/> .
@prefix dct: <http://purl.org/dc/terms/> .
@prefix eu-nis2: <https://w3id.org/dpv/legal/eu/nis2#> .
@prefix foaf: <http://xmlns.com/foaf/0.1/> .
@prefix owl: <http://www.w3.org/2002/07/owl#> .
@prefix profile: <http://www.w3.org/ns/dx/prof/> .
@prefix rdf: <http://www.w3.org/1999/02/22-rdf-syntax-ns#> .
@prefix rdfs: <http://www.w3.org/2000/01/rdf-schema#> .
@prefix risk: <https://w3id.org/dpv/risk#> .
@prefix role: <http://www.w3.org/ns/dx/prof/role/> .
@prefix schema: <https://schema.org/> .
@prefix skos: <http://www.w3.org/2004/02/skos/core#> .
@prefix sw: <http://www.w3.org/2003/06/sw-vocab-status/ns#> .
@prefix vann: <http://purl.org/vocab/vann/> .
@prefix xsd: <http://www.w3.org/2001/XMLSchema#> .

eu-nis2:EarlyWarningReport a rdfs:Class,
        skos:Concept,
        risk:IncidentNotice ;
    dct:contributor "Harshvardhan J. Pandit, Georg P. Krog" ;
    dct:created "2024-05-19"^^xsd:date ;
    dct:source "NIS2 Directive"@en ;
    rdfs:isDefinedBy eu-nis2: ;
    sw:term_status "accepted"@en ;
    skos:broader risk:IncidentNotice ;
    skos:definition "within 24 hours of detection containing cause of the  incident and whether it was unlawful or malicious and whether there is  cross-border impact"@en ;
    skos:inScheme eu-nis2:notice-classes ;
    skos:prefLabel "Early Warning Report"@en .

eu-nis2:FinalReport a rdfs:Class,
        skos:Concept,
        risk:IncidentNotice ;
    dct:contributor "Harshvardhan J. Pandit, Georg P. Krog" ;
    dct:created "2024-05-19"^^xsd:date ;
    dct:source "NIS2 Directive"@en ;
    rdfs:isDefinedBy eu-nis2: ;
    sw:term_status "accepted"@en ;
    skos:broader risk:IncidentNotice ;
    skos:definition "within 1 month of incident handling i.e.  completing the incident recovery and containing the  applied/ongoing measures, 'detailed description' - not sure what this  means, and threat type / root cause - which is covered with threat and  vulnerability concepts"@en ;
    skos:inScheme eu-nis2:notice-classes ;
    skos:prefLabel "Final Report"@en .

eu-nis2:IncidentAssessmentReport a rdfs:Class,
        skos:Concept,
        risk:IncidentNotice ;
    dct:contributor "Harshvardhan J. Pandit, Georg P. Krog" ;
    dct:created "2024-05-19"^^xsd:date ;
    dct:source "NIS2 Directive"@en ;
    rdfs:isDefinedBy eu-nis2: ;
    sw:term_status "accepted"@en ;
    skos:broader risk:IncidentNotice ;
    skos:definition "within 72 hours of detection, which contains  updates on the earlier information as well as initial assessment of  severity and impact of the incident as well as any 'indicators of  compromise'"@en ;
    skos:inScheme eu-nis2:notice-classes ;
    skos:prefLabel "Incident Assessment Report"@en .

eu-nis2:InitialFeedbackOnIncident a rdfs:Class,
        skos:Concept,
        risk:IncidentNotice ;
    dct:contributor "Harshvardhan J. Pandit, Georg P. Krog" ;
    dct:created "2024-05-19"^^xsd:date ;
    dct:source "NIS2 Directive"@en ;
    rdfs:isDefinedBy eu-nis2: ;
    sw:term_status "accepted"@en ;
    skos:broader risk:IncidentNotice ;
    skos:definition "Notification from authority to organisation (upon request, within 24 hours or early warning) containing  \"initial feedback\" and guidelines on measures that can be taken in  response to a breach"@en ;
    skos:inScheme eu-nis2:notice-classes ;
    skos:prefLabel "Initial Feedback on Incident"@en .

eu-nis2:IntermediateReport a rdfs:Class,
        skos:Concept,
        risk:IncidentNotice ;
    dct:contributor "Harshvardhan J. Pandit, Georg P. Krog" ;
    dct:created "2024-05-19"^^xsd:date ;
    dct:source "NIS2 Directive"@en ;
    rdfs:isDefinedBy eu-nis2: ;
    sw:term_status "accepted"@en ;
    skos:broader risk:IncidentNotice ;
    skos:definition "upon request - which provides updates, if any,  to previous information"@en ;
    skos:inScheme eu-nis2:notice-classes ;
    skos:prefLabel "Intermediate Report"@en .

eu-nis2:ProgressReport a rdfs:Class,
        skos:Concept,
        risk:IncidentNotice ;
    dct:contributor "Harshvardhan J. Pandit, Georg P. Krog" ;
    dct:created "2024-05-19"^^xsd:date ;
    dct:source "NIS2 Directive"@en ;
    rdfs:isDefinedBy eu-nis2: ;
    sw:term_status "accepted"@en ;
    skos:broader risk:IncidentNotice ;
    skos:definition "within 1 month of detection if the  incident handling has not been completed by then, with updates to  previous information"@en ;
    skos:inScheme eu-nis2:notice-classes ;
    skos:prefLabel "Progress Report"@en .

eu-nis2:RiskMitigationAdvice a rdfs:Class,
        skos:Concept,
        risk:IncidentNotice ;
    dct:contributor "Harshvardhan J. Pandit, Georg P. Krog" ;
    dct:created "2024-05-19"^^xsd:date ;
    dct:source "NIS2 Directive"@en ;
    rdfs:isDefinedBy eu-nis2: ;
    sw:term_status "accepted"@en ;
    skos:broader risk:IncidentNotice ;
    skos:definition "Notification from organisation to stakeholders regarding risk mitigations to be applied and existence of threats"@en ;
    skos:inScheme eu-nis2:notice-classes ;
    skos:prefLabel "Risk Mitigation Advice"@en .

eu-nis2:SignificantIncidentNotice a rdfs:Class,
        skos:Concept ;
    dct:contributor "Harshvardhan J. Pandit, Georg P. Krog" ;
    dct:created "2024-05-19"^^xsd:date ;
    dct:source "NIS2 Directive"@en ;
    rdfs:isDefinedBy eu-nis2: ;
    rdfs:subClassOf risk:IncidentNotice ;
    sw:term_status "accepted"@en ;
    skos:broader risk:IncidentNotice ;
    skos:definition "Notice sent for reporting significant incidents"@en ;
    skos:inScheme eu-nis2:notice-classes ;
    skos:prefLabel "Significant Incident Notice"@en .

<https://w3id.org/dpv/legal/eu/nis2> a owl:Ontology,
        profile:Profile ;
    dct:bibliographicCitation "Data Privacy Vocabulary (DPV) -- Version 2. Harshvardhan J. Pandit, Beatriz Esteves, Georg P. Krog, Paul Ryan, Delaram Golpayegani, Julian Flake https://doi.org/10.48550/arXiv.2404.13426" ;
    dct:conformsTo "http://www.w3.org/2000/01/rdf-schema",
        "http://www.w3.org/2004/02/skos/core" ;
    dct:contributor "Georg P. Krog",
        "Harshvardhan J. Pandit" ;
    dct:created "2024-05-19"@en ;
    dct:creator "Georg P. Krog"@en,
        "Harshvardhan J. Pandit"@en ;
    dct:description "Extension to the Data Privacy Vocabulary (DPV) providing concepts for representing  information associated with EU NIS2"@en ;
    dct:identifier "https://w3id.org/dpv/legal/eu/nis2" ;
    dct:issued "2024-05-19"@en ;
    dct:license <https://www.w3.org/copyright/document-license-2023/> ;
    dct:modified "2024-07-01"@en ;
    dct:publisher <https://www.w3.org/> ;
    dct:source <https://www.w3.org/groups/cg/dpvcg/> ;
    dct:title "EU NIS2"@en ;
    bibo:doi "10.5281/zenodo.12505841" ;
    bibo:status "http://purl.org/ontology/bibo/status/published" ;
    vann:preferredNamespacePrefix "eu-nis2" ;
    vann:preferredNamespaceUri "https://w3id.org/dpv/legal/eu/nis2#" ;
    rdfs:Label "EU-NIS2"@en ;
    owl:versionIRI <https://w3id.org/dpv/2.0/legal/eu/nis2> ;
    owl:versionInfo "2.0" ;
    profile:hasResource <https://w3id.org/dpv/examples>,
        <https://w3id.org/dpv/guides>,
        eu-nis2:serialisation-html,
        eu-nis2:serialisation-jsonld,
        eu-nis2:serialisation-n3,
        eu-nis2:serialisation-rdf,
        eu-nis2:serialisation-ttl,
        <https://w3id.org/dpv/primer> ;
    profile:isProfileOf rdfs:,
        skos:,
        <https://w3id.org/dpv> ;
    foaf:logo <https://w3id.org/dpv/media/logo.png> ;
    schema:version "2.0" .

eu-nis2:serialisation-html a profile:ResourceDescriptor ;
    dct:conformsTo <https://www.w3.org/TR/html/> ;
    dct:format <https://www.iana.org/assignments/media-types/text/html> ;
    dct:title "EU NIS2 - HTML serialiation" ;
    profile:hasArtifact <https://w3id.org/dpv/legal/eu/nis2/eu-nis2.html> ;
    profile:hasRole role:specification .

eu-nis2:serialisation-jsonld a profile:ResourceDescriptor ;
    dct:conformsTo <https://www.w3.org/TR/json-ld11/> ;
    dct:format <https://www.iana.org/assignments/media-types/application/ld+json> ;
    dct:title "EU NIS2 - JSON-LD serialiation" ;
    profile:hasArtifact <https://w3id.org/dpv/legal/eu/nis2/eu-nis2.jsonld> ;
    profile:hasRole role:vocabulary .

eu-nis2:serialisation-n3 a profile:ResourceDescriptor ;
    dct:conformsTo <https://www.w3.org/TeamSubmission/n3/> ;
    dct:format <https://www.iana.org/assignments/media-types/text/n3> ;
    dct:title "EU NIS2 - N3 serialiation" ;
    profile:hasArtifact <https://w3id.org/dpv/legal/eu/nis2/eu-nis2.n3> ;
    profile:hasRole role:vocabulary .

eu-nis2:serialisation-rdf a profile:ResourceDescriptor ;
    dct:conformsTo rdf: ;
    dct:format <https://www.iana.org/assignments/media-types/application/rdf+xml> ;
    dct:title "EU NIS2 - RDF/XML serialiation" ;
    profile:hasArtifact <https://w3id.org/dpv/legal/eu/nis2/eu-nis2.rdf> ;
    profile:hasRole role:vocabulary .

eu-nis2:serialisation-ttl a profile:ResourceDescriptor ;
    dct:conformsTo <https://www.w3.org/TR/turtle/> ;
    dct:format <https://www.iana.org/assignments/media-types/text/turtle> ;
    dct:title "EU NIS2 - Turtle serialiation" ;
    profile:hasArtifact <https://w3id.org/dpv/legal/eu/nis2/eu-nis2.ttl> ;
    profile:hasRole role:vocabulary .

<https://w3id.org/dpv/examples> a profile:ResourceDescriptor ;
    dct:conformsTo <https://www.w3.org/TR/html/> ;
    dct:format <https://www.iana.org/assignments/media-types/text/html> ;
    dct:title "Examples for Data Privacy Vocabulary" ;
    profile:hasArtifact <https://w3id.org/dpv/examples> ;
    profile:hasRole role:guidance .

<https://w3id.org/dpv/guides> a profile:ResourceDescriptor ;
    dct:conformsTo <https://www.w3.org/TR/html/> ;
    dct:format <https://www.iana.org/assignments/media-types/text/html> ;
    dct:title "Guides for Data Privacy Vocabulary" ;
    profile:hasArtifact <https://w3id.org/dpv/guides> ;
    profile:hasRole role:guidance .

<https://w3id.org/dpv/primer> a profile:ResourceDescriptor ;
    dct:conformsTo <https://www.w3.org/TR/html/> ;
    dct:format <https://www.iana.org/assignments/media-types/text/html> ;
    dct:title "Primer for Data Privacy Vocabulary" ;
    profile:hasArtifact <https://w3id.org/dpv/primer> ;
    profile:hasRole role:guidance .

eu-nis2:notice-classes a skos:ConceptScheme .

